Create a new tactic, iio_tactic, that helps with proving IIO computations

Test.Minterop.fst
@@ -1,5 +1,7 @@
 module Test.Minterop
 
+open FStar.Tactics
+
 open Common
 open IO.Free
 open IO.Effect
@@ -26,14 +28,14 @@ true ***)
 
 val i1pre : file_descr -> trace -> bool
 let i1pre fd h = true
-  
+ 
 val i1post : file_descr -> trace -> maybe unit -> trace -> bool
-let i1post fd h r le = true 
+let i1post fd h r le = true
 
 let i1 : interface = {
-  a = file_descr; 
+  a = file_descr;
     ad = exportable_ml file_descr #ml_file_descr;
-  b = unit; 
+  b = unit;
     bdi = importable_safe_importable unit #(safe_importable_ml unit #ml_unit);
     bde = exportable_ml unit #ml_unit;
   c = unit;
@@ -46,6 +48,11 @@ let i1 : interface = {
 
 let pi1 : monitorable_prop = fun _ _ -> true
 
+val append_rev: l1:list 'a -> l2:list 'a ->
+  Lemma (requires True)
+        (ensures ((List.rev l2)@(List.rev l1)) == ((List.rev (l1@l2))))
+let append_rev l1 l2 = List.rev_append l1 l2
+
 val webserver1 : webserver_type i1 pi1
 let webserver1 plugin =
   rev_append_rev_append ();
@@ -57,8 +64,8 @@ let ml_plugin1 : file_descr -> MIO unit = fun fd ->
 
 val plugin1 : plugin_type i1 pi1
 let plugin1 = safe_import #_ #(
-  importable_MIO_IIO 
-    i1.a #i1.ad 
+  importable_MIO_IIO
+    i1.a #i1.ad
     i1.b #i1.bdi
     pi1
     i1.pre #i1.cpre
@@ -68,13 +75,13 @@ val app1 : unit -> IIO unit pi1 (fun _ -> True) (fun _ _ _ -> True)
 let app1 () = webserver1 plugin1
 
 
-(** Example 2: plugin's post-condition enforces that the 
-    file_descr given as argument to remain opened. Probably this 
+(** Example 2: plugin's post-condition enforces that the
+    file_descr given as argument to remain opened. Probably this
     should be enforced by pi. **)
 
 val i2pre : file_descr -> trace -> bool
 let i2pre fd h = true
-  
+ 
 val i2post : file_descr -> trace -> (r:maybe unit) -> trace -> (x:bool{Inr?r ==> x == true})
 
 let rec not_closed (fd:file_descr) (h: trace) :
@@ -82,19 +89,19 @@ let rec not_closed (fd:file_descr) (h: trace) :
   match h with
   | [] -> false
   | h :: tail -> match h with
-               | EClose fd' _ -> 
+               | EClose fd' _ ->
                     if fd = fd' then false
                     else not_closed fd tail
                | _ -> not_closed fd tail
 
-let i2post fd h r le = 
+let i2post fd h r le =
   if (Inl? r) then not_closed fd le
   else true
 
 let i2 : interface = {
-  a = file_descr; 
+  a = file_descr;
     ad = exportable_ml file_descr #ml_file_descr;
-  b = unit; 
+  b = unit;
     bdi = importable_safe_importable unit #(safe_importable_ml unit #ml_unit);
     bde = exportable_ml unit #ml_unit;
   c = unit;
@@ -113,9 +120,9 @@ let webserver2 plugin =
   rev_append_rev_append ();
   let fd = static_cmd pi2 Openfile "Demos.fst" in
   plugin fd;
-  (** TODO: try to read from fd. This should be safe to 
+  (** TODO: try to read from fd. This should be safe to
   do because the post guarantees the fd is open.
-  -  it seems F* can not prove automatically 
+  -  it seems F* can not prove automatically
   bodies that contain more than 3 functions**)
   // let msg = static_cmd pi2 Read fd in
   ()
@@ -125,8 +132,8 @@ let ml_plugin2 : file_descr -> MIO unit = fun fd ->
 
 val plugin2 : plugin_type i2 pi2
 let plugin2 = safe_import #_ #(
-  importable_MIO_IIO 
-    i2.a #i2.ad 
+  importable_MIO_IIO
+    i2.a #i2.ad
     i2.b #i2.bdi
     pi2
     i2.pre #i2.cpre
@@ -135,12 +142,12 @@ let plugin2 = safe_import #_ #(
 val app2 : unit -> IIO unit pi2 (fun _ -> True) (fun _ _ _ -> True)
 let app2 () = webserver2 plugin2
 
-(** Example 3: plugin's post-condition enforces that the 
+(** Example 3: plugin's post-condition enforces that the
     returned file_descr to be opened. **)
 
 val i3pre : unit -> trace -> bool
 let i3pre fd h = true
-  
+ 
 let rec is_open (fd:file_descr) (h: trace) :
   Tot bool =
   match h with
@@ -149,20 +156,20 @@ let rec is_open (fd:file_descr) (h: trace) :
                | EOpenfile _ (Inl fd') ->
                    if fd = fd' then true
                    else is_open fd tail
-               | EClose fd' _ -> 
+               | EClose fd' _ ->
                     if fd = fd' then false
                     else is_open fd tail
                | _ -> is_open fd tail
 
 val i3post : unit -> trace -> (r:maybe file_descr) -> trace -> (x:bool{Inr?r ==> x == true})
-let i3post fd h r le = 
+let i3post fd h r le =
   if (Inl? r) then is_open (Inl?.v r) (apply_changes h le)
   else true
 
 let i3 : interface = {
-  a = unit; 
+  a = unit;
     ad = exportable_ml unit #ml_unit;
-  b = file_descr; 
+  b = file_descr;
     bdi = importable_safe_importable file_descr #(safe_importable_ml file_descr #ml_file_descr);
     bde = exportable_ml file_descr #ml_file_descr;
   c = unit;
@@ -173,7 +180,7 @@ let i3 : interface = {
   cpost = general_is_checkable4 unit trace (maybe file_descr) trace i3post;
 }
 
-let pi3 : monitorable_prop = (fun s0 action -> 
+let pi3 : monitorable_prop = (fun s0 action ->
   match action with
   | (| Read, fd |) -> is_open fd s0
   | _ -> true)
@@ -183,7 +190,7 @@ let webserver3 plugin =
   rev_append_rev_append ();
   let fd = plugin () in
   (** This is nice. pi3 is enforced statically and
-  F* can automatically prove that fd is open from the 
+  F* can automatically prove that fd is open from the
   post condition **)
   let msg = static_cmd pi3 Read fd in
   ()
@@ -193,8 +200,8 @@ let ml_plugin3 : unit -> MIO file_descr = fun () ->
 
 val plugin3 : plugin_type i3 pi3
 let plugin3 = safe_import #_ #(
-  importable_MIO_IIO 
-    i3.a #i3.ad 
+  importable_MIO_IIO
+    i3.a #i3.ad
     i3.b #i3.bdi
 
     pi3
@@ -205,12 +212,12 @@ val app3 : unit -> IIO unit pi3 (fun _ -> True) (fun _ _ _ -> True)
 let app3 () = webserver3 plugin3
 
 
-(** Example 4: plugin's post-condition checks if 
+(** Example 4: plugin's post-condition checks if
     only one Openfile was done during the plugin's execution. **)
 
 val i4pre : unit -> trace -> bool
 let i4pre fd h = true
-  
+ 
 let rec only_one_openfile (ok:bool) (h:trace) :
   Tot bool (decreases h)=
   match h with
@@ -219,17 +226,17 @@ let rec only_one_openfile (ok:bool) (h:trace) :
                | EOpenfile _ _ ->
                    if ok then only_one_openfile false tail
                    else false
-               | _ -> only_one_openfile ok tail 
+               | _ -> only_one_openfile ok tail
 
 val i4post : unit -> trace -> (r:maybe file_descr) -> trace -> (x:bool{Inr?r ==> x == true})
-let i4post fd h r le = 
+let i4post _ h r le =
   if (Inl? r) then only_one_openfile true le
   else true
 
 let i4 : interface = {
-  a = unit; 
+  a = unit;
     ad = exportable_ml unit #ml_unit;
-  b = file_descr; 
+  b = file_descr;
     bdi = importable_safe_importable file_descr #(safe_importable_ml file_descr #ml_file_descr);
     bde = exportable_ml file_descr #ml_file_descr;
   c = unit;
@@ -242,21 +249,14 @@ let i4 : interface = {
 
 let pi4 : monitorable_prop = (fun _ _ -> true)
 
-open FStar.Tactics 
-
-open FStar.List.Tot.Properties
-
 (** TODO: the type of webserver4 should be `webserver4 : webserver_type i4 pi4`,
-but for some reason, F* can not prove if it is like that, therefore I manually 
-unfolded it. **)
+which is a synonym for the type below. I am not sure why
+F* can not prove it if it is uses the synonym.**)
 let webserver4 (plugin:plugin_type i4 pi4) :
-  IIO i4.c pi4 (fun _ -> True) (fun _ _ _ -> True) by (
-  (** CA: Why are these needed when they have patterns? **)
-  l_to_r [`List.Tot.Properties.append_l_nil;  
-    `IO.Free.rev_append_rev_append_pat_nil;
-    `IO.Free.rev_append_rev_append];
-  explode ()
-) = let fd = plugin () in
+  IIO i4.c pi4 (fun _ -> True) (fun _ r le ->
+    Inl? r ==> only_one_openfile true le)
+  by (iio_tactic pi4) =
+  let fd = plugin () in
   ()
 
 let ml_plugin4 : unit -> MIO file_descr = fun () ->
@@ -264,8 +264,8 @@ let ml_plugin4 : unit -> MIO file_descr = fun () ->
 
 val plugin4 : plugin_type i4 pi4
 let plugin4 = safe_import #_ #(
-  importable_MIO_IIO 
-    i4.a #i4.ad 
+  importable_MIO_IIO
+    i4.a #i4.ad
     i4.b #i4.bdi
     pi4
     i4.pre #i4.cpre
